Filling out trait and enumerator adaptor

TestModels/dafny-dependencies/StandardLibrary/src/Streams.dfy
@@ -1,33 +1,180 @@
 
-module StandardLibrary.Streams {
+module {:options "--function-syntax:4"} StandardLibrary.Streams {
 
   import opened Std.Wrappers
+  import opened Std.Actions
   import opened Std.Enumerators
   import opened Std.BoundedInts
+  import opened Std.Collections.Seq
 
-  trait DataStream extends Enumerator<bytes> {
+  // Alias just for clarity
+  type EventStream<T> = Enumerator<T>
+
+  trait DataStream extends Enumerator<BoundedInts.bytes> {
 
     ghost const value: bytes
-    ghost var contentLength: uint64
-    ghost var position: uint64
-    ghost var mark: Option<uint64>
 
-    function ContentLength(): Option<uint64>
+    ghost predicate Valid() 
+      reads this, Repr 
+      ensures Valid() ==> this in Repr 
+      ensures Valid() ==> CanProduce(history)
+      decreases height, 0
 
-    predicate SupportsMarkAndReset()
+    function ConcatenatedOutputs(history: seq<((), Option<bytes>)>): bytes {
+      Flatten(Enumerated(Outputs(history)))
+    }
 
-    method Mark() 
-      requires SupportsMarkAndReset()
-      requires mark.None?
-      ensures mark == Some(position)
+    function ContentLength(): (res: Option<uint64>)
+      requires Valid()
+      reads this, Repr
+      ensures res.Some? ==> res.value as int == |value|
 
-    method Reset()
-      requires SupportsMarkAndReset()
-      requires mark.Some?
-      ensures position == mark.value
+    ghost predicate CanProduce(history: seq<((), Option<bytes>)>)
+      decreases height
+    {
+      && (forall o <- Enumerated(Outputs(history)) :: 0 < |o|)
+      && ConcatenatedOutputs(history) <= value
+    }
 
-    // TODO: the rest of the fudging owl
+    lemma {:axiom} ProducesTerminated(history: seq<((), Option<bytes>)>)
+      requires Action().CanProduce(history) 
+      requires (forall i <- Inputs(history) :: i == FixedInput())
+      ensures exists n: nat | n <= Limit() :: Terminated(Outputs(history), StopFn(), n)
+    // {
+    //   assert Terminated(Outputs(history), StopFn(), |Enumerated(Outputs(history))|);
+    // }
+
+    method RepeatUntil(t: (), stop: Option<bytes> -> bool, ghost eventuallyStopsProof: ProducesTerminatedProof<(), Option<bytes>>)
+      requires Valid()
+      requires eventuallyStopsProof.Action() == this
+      requires eventuallyStopsProof.FixedInput() == t
+      requires eventuallyStopsProof.StopFn() == stop
+      requires forall i <- Consumed() :: i == t
+      modifies Repr
+      decreases Repr
+      ensures Valid()
+    {
+      DefaultRepeatUntil(this, t, stop, eventuallyStopsProof);
+    }
+
+    /*
+     * Whether this stream can be read multiple times.
+     * If this is true, it is at least possible to seek to earlier positions.
+     * This does not necessarily mean seeking is constant time,
+     * because it may mean re-reading from the start of the stream.
+     */
+    predicate Rewindable()
+      decreases height, 1
+
+    function Position(): (res: uint64)
+      requires Valid()
+      requires Rewindable()
+      reads this, Repr
+      decreases height, 2
+      ensures res as int <= |value|
+
+    method Seek(newPosition: uint64)
+      requires Valid()
+      requires Rewindable()
+      requires newPosition as int <= |value|
+      ensures Valid()
+      ensures Position() == newPosition
   }
 
-  type EventStream<T> = Enumerator<T>
+  /*
+   * Wraps an Enumerator up as a non-rewindable DataStream.
+   */
+  class EnumeratorDataStream<bytes> extends DataStream {
+
+    const wrapped: Enumerator<BoundedInts.bytes>
+    const length: Option<uint64>
+
+    ghost predicate Valid() 
+      reads this, Repr 
+      ensures Valid() ==> this in Repr 
+      ensures Valid() ==> CanProduce(history)
+      decreases height, 0
+    {
+      && this in Repr
+      && ValidComponent(wrapped)
+      && CanProduce(history)
+      && (length.Some? ==> length.value as int == |value|)
+    }
+
+    lemma {:axiom} ProducesTerminated(history: seq<((), Option<BoundedInts.bytes>)>)
+      requires Action().CanProduce(history) 
+      requires (forall i <- Inputs(history) :: i == FixedInput())
+      ensures exists n: nat | n <= Limit() :: Terminated(Outputs(history), StopFn(), n)
+
+    ghost function Limit(): nat {
+      wrapped.Limit()
+    }
+
+    constructor(wrapped: Enumerator<BoundedInts.bytes>, length: Option<uint64>, ghost value: BoundedInts.bytes) 
+      requires wrapped.Valid()
+      requires wrapped.history == []
+      requires length.Some? ==> length.value as int == |value|
+      ensures Valid()
+    {
+      this.wrapped := wrapped;
+      this.length := length;
+      this.value := value;
+
+      this.history := [];
+      this.Repr := {this} + wrapped.Repr;
+      this.height := wrapped.height + 1;
+    }
+
+    function ContentLength(): (res: Option<uint64>)
+      requires Valid()
+      reads this, Repr
+      ensures res.Some? ==> res.value as int == |value|
+    {
+      length
+    }
+
+    predicate Rewindable()
+      decreases height, 1
+    {
+      false
+    }
+
+    function Position(): (res: uint64)
+      requires Rewindable()
+      reads this, Repr
+      ensures res as int <= |value|
+    {
+      // Unreachable
+      assert false;
+      0
+    }
+
+    method Seek(newPosition: uint64)
+      requires Valid()
+      requires Rewindable()
+      requires newPosition as int <= |value|
+      ensures Valid()
+      ensures Position() == newPosition
+    {
+      // Unreachable
+      assert false;
+    }
+
+    method Invoke(t: ()) returns (r: Option<BoundedInts.bytes>) 
+      requires Requires(t)
+      modifies Modifies(t)
+      decreases Decreases(t).Ordinal()
+      ensures Ensures(t, r)
+    {
+      // TODO: Not sure why this isn't provable from GenericAction?
+      assume {:axiom} Valid();
+      r := wrapped.Next();
+      Update(t, r);
+      
+      // TODO: Work to do
+      assume {:axiom} Ensures(t, r);
+    }
+  }
+
+
 }
